
-- {-# OPTIONS --cubical --allow-unsolved-metas #-}

module Verification.Conventions.Prelude.Classes.EquivalenceRelation where

open import Verification.Conventions.Proprelude
open import Verification.Conventions.Prelude.Classes.Operators.Unary
open import Verification.Conventions.Prelude.Classes.Cast
open import Verification.Conventions.Prelude.Classes.Anything
open import Verification.Conventions.Prelude.Data.StrictId
open import Verification.Conventions.Prelude.Classes.Setoid
-- open import Verification.Conventions.Prelude.Data.Product


--------------------------------------------------------------------------------
-- == Equivalence relation
--






-- [Definition]
record isEquivRel {X : ğ’° ğ‘–} (_â‰£_ : X -> X -> ğ’° ğ‘—) : ğ’° (ğ‘– âŠ” ğ‘—) where
  constructor equivRel
  field refl-Equiv : âˆ€{x : X} -> x â‰£ x
        sym-Equiv : âˆ€{x y : X} -> x â‰£ y -> y â‰£ x
        _âˆ™-Equiv_ : âˆ€{x y z : X} -> x â‰£ y -> y â‰£ z -> x â‰£ z

  infixl 30 _âˆ™-Equiv_
open isEquivRel {{...}} public
-- //

-- module _ {X : ğ’° ğ‘–} {_â‰£_ : X -> X -> ğ’° ğ‘—} {{_ : isEquivRel _â‰£_}} where
--   instance
--     Notation-Inverse:Equiv : {x y : X} -> Notation-Inverse (x â‰£ y) (y â‰£ x)
--     Notation-Inverse:Equiv Notation-Inverse.â»Â¹ = sym




infixl 10 >><<-syntax
>><<-syntax : âˆ€(A : ğ’° ğ‘–) -> A -> A
>><<-syntax A a = a
syntax >><<-syntax A a = a >> A <<

infixl 10 âŸªâŸ«-syntax
âŸªâŸ«-syntax : âˆ€{A : ğ’° ğ‘–} {B : ğ’° ğ‘—} -> A -> (A -> B) -> B
âŸªâŸ«-syntax a f = f a
syntax âŸªâŸ«-syntax a f = a âŸª f âŸ«


module _ {A : ğ’° ğ‘–} {{_ : isSetoid {ğ‘—} A}} where
  both : {a b c d : A} -> (a âˆ¼ c) -> (b âˆ¼ d) -> a âˆ¼ b -> c âˆ¼ d
  both p q r = p â»Â¹ âˆ™ r âˆ™ q


_â‰€âˆ¼â‰€_ = both






  -- setoid _â‰£_ refl-â‰£ (Î» {refl-â‰£ -> refl-â‰£}) (Î»{refl-â‰£ q -> q})

-- instance
-- module _ where
  -- isEquivRel:Path : {X : ğ’° ğ‘–} -> isEquivRel (Î» (x y : X) -> x â‰¡ y)
  -- isEquivRel.refl  isEquivRel:Path = refl-Path
  -- isEquivRel.sym   isEquivRel:Path = sym-Path
  -- isEquivRel._âˆ™_   isEquivRel:Path = trans-Path


-- module _ {X : ğ’° ğ‘–} (_âˆ¼_ : X -> X -> ğ’° ğ‘—) where
--   record hasTransport : ğ’° ğ‘— where
--     field transport : âˆ€{a b : X} (a âˆ¼ b) -> 



-- module _ {X : ğ’° ğ‘–} {_âˆ¼_ : X -> X -> ğ’° ğ‘—} {{_ : isEquivRel _âˆ¼_}} where
--   fromPath : âˆ€{a b : X} -> a â‰¡ b -> a âˆ¼ b
--   fromPath {a = a} p = transport (Î» i -> a âˆ¼ p i) refl

-- sym-Id : âˆ€{X : ğ’° ğ‘–} {x y : X} -> Id x y -> Id y x
-- sym-Id {x = x} {y = y} p = J-Id (Î» y _ -> Id y x) refl-Id p

{-
trans-Id : âˆ€{X : ğ’° ğ‘–} {x y z : X} -> Id x y -> Id y z -> Id x z
trans-Id {x = x} {y} {z} p q = J-Id (Î» z _ -> Id x z) p q

instance
-- module _ where
  isEquivRel:Id : {X : ğ’° ğ‘–} -> isEquivRel (Î» (x y : X) -> Id x y)
  isEquivRel.refl isEquivRel:Id = refl-Id
  isEquivRel.sym isEquivRel:Id = sym-Id
  isEquivRel._âˆ™_ isEquivRel:Id = trans-Id

module _ {X : ğ’° ğ‘˜} {x : X} where
  record âˆ€Id (P : (y : X) -> Id x y -> ğ’° ğ‘™) : ğ’° (ğ‘˜ âŠ” ğ‘™) where
    constructor idproof
    field getProof : âˆ€{y : X} -> (p : Id x y) -> P y p

  open âˆ€Id public

  J-âˆ€Id : âˆ€{P : (y : X) -> Id x y -> ğ’° ğ‘™} -> (d : P x refl-Id) -> âˆ€Id P
  J-âˆ€Id {P = P} d = idproof $ Î» p -> (J-Id P d p)

congâ‚‚-Id-helper : âˆ€{A : ğ’° ğ‘–} {B : ğ’° ğ‘—} {C : ğ’° ğ‘˜} -> {a1 : A} {b1 : B} -> (f : A -> B -> C)
                 -> âˆ€Id (Î» a2 (p : Id a1 a2) -> âˆ€Id (Î» b2 (q : Id b1 b2) -> Id (f a1 b1) (f a2 b2)))
congâ‚‚-Id-helper f = J-âˆ€Id (J-âˆ€Id refl-Id)

congâ‚‚-Id : âˆ€{A : ğ’° ğ‘–} {B : ğ’° ğ‘—} {C : ğ’° ğ‘˜} -> {a1 a2 : A} {b1 b2 : B} -> (f : A -> B -> C) -> (Id a1 a2) -> (Id b1 b2) -> Id (f a1 b1) (f a2 b2)
congâ‚‚-Id f p q = congâ‚‚-Id-helper f .getProof p .getProof q
-}

-- instance
-- module _ where
  -- isEquivRel:StrId : {X : ğ’° ğ‘–} -> isEquivRel (Î» (x y : X) -> StrId x y)
  -- isEquivRel.refl isEquivRel:StrId = refl-StrId
  -- isEquivRel.sym isEquivRel:StrId refl-StrId = refl-StrId
  -- (isEquivRel:StrId isEquivRel.âˆ™ refl-StrId) q = q


instance
  Cast:â‰¡Str : âˆ€{X : ğ’° ğ‘–} -> âˆ€{a b : X} -> Cast (a â‰¡-Str b) IAnything (a â‰¡ b)
  Cast.cast Cast:â‰¡Str refl-StrId = refl-Path

â‰¡-Strâ†’â‰¡ : âˆ€{X : ğ’° ğ‘–} -> âˆ€{a b : X} -> (a â‰¡-Str b) -> (a â‰¡ b)
â‰¡-Strâ†’â‰¡ refl-StrId = refl-Path

â‰¡â†’â‰¡-Str : âˆ€{X : ğ’° ğ‘–} -> âˆ€{a b : X} -> (a â‰¡ b) -> (a â‰¡-Str b)
â‰¡â†’â‰¡-Str {a = a} {b} p = transport (Î» i -> a â‰¡-Str (p i)) refl-StrId

-- rightâ‰¢left-Str : âˆ€{a : A}

â‰¡-change-iso : âˆ€{X : ğ’° ğ‘–} -> âˆ€{a b : X} -> (p : a â‰¡-Str b) -> (â‰¡â†’â‰¡-Str (â‰¡-Strâ†’â‰¡ p) â‰¡ p)
â‰¡-change-iso refl-StrId = transportRefl refl-StrId

--------------------------------------------------------------------------------
-- === path syntax

module _ {A : ğ’° ğ‘–} {{_ : isSetoid {ğ‘—} A}} where
  _â‰£âŸ¨_âŸ©_ : (x : A) {y : A} {z : A} â†’ x âˆ¼ y â†’ y âˆ¼ z â†’ x âˆ¼ z
  _ â‰£âŸ¨ xâ‰¡y âŸ© yâ‰¡z = xâ‰¡y âˆ™ yâ‰¡z

  â‰£âŸ¨âŸ©-syntax : (x : A) {y z : A} â†’ x âˆ¼ y â†’ y âˆ¼ z â†’ x âˆ¼ z
  â‰£âŸ¨âŸ©-syntax = _â‰£âŸ¨_âŸ©_
  infixr 2 â‰£âŸ¨âŸ©-syntax
  infix  3 _âˆ
  infixr 2 _â‰£âŸ¨_âŸ©_

  _âˆ : (x : A) â†’ x âˆ¼ x
  _ âˆ = refl


-- new syntax with âˆ¼
module _ {A : ğ’° ğ‘–} {{_ : isSetoid {ğ‘—} A}} where
  _âŸ¨_âŸ©-âˆ¼_ : (x : A) {y : A} {z : A} â†’ x âˆ¼ y â†’ y âˆ¼ z â†’ x âˆ¼ z
  _ âŸ¨ xâ‰¡y âŸ©-âˆ¼ yâ‰¡z = xâ‰¡y âˆ™ yâ‰¡z

  âŸ¨âŸ©-âˆ¼-syntax : (x : A) {y z : A} â†’ x âˆ¼ y â†’ y âˆ¼ z â†’ x âˆ¼ z
  âŸ¨âŸ©-âˆ¼-syntax = _âŸ¨_âŸ©-âˆ¼_
  infixr 2 âŸ¨âŸ©-âˆ¼-syntax
  infixr 2 _âŸ¨_âŸ©-âˆ¼_

  infix  3 _âˆ-âˆ¼

  _âˆ-âˆ¼ : (x : A) â†’ x âˆ¼ x
  _ âˆ-âˆ¼ = refl


module _ {A : ğ’° ğ‘–} where
  _âŸ¨_âŸ©-â‰¡_ : (x : A) {y : A} {z : A} â†’ x â‰¡ y â†’ y â‰¡ z â†’ x â‰¡ z
  _ âŸ¨ xâ‰¡y âŸ©-â‰¡ yâ‰¡z = trans-Path xâ‰¡y yâ‰¡z

  âŸ¨âŸ©-â‰¡-syntax : (x : A) {y z : A} â†’ x â‰¡ y â†’ y â‰¡ z â†’ x â‰¡ z
  âŸ¨âŸ©-â‰¡-syntax = _âŸ¨_âŸ©-â‰¡_
  infixr 2 âŸ¨âŸ©-â‰¡-syntax
  infixr 2 _âŸ¨_âŸ©-â‰¡_

  infix  3 _âˆ-â‰¡

  _âˆ-â‰¡ : (x : A) â†’ x â‰¡ x
  _ âˆ-â‰¡ = refl-â‰¡

module _ {A : ğ’° ğ‘–} where
  _âŸ¨_âŸ©-â‰£_ : (x : A) {y : A} {z : A} â†’ x â‰£ y â†’ y â‰£ z â†’ x â‰£ z
  _ âŸ¨ xâ‰£y âŸ©-â‰£ yâ‰£z =  xâ‰£y âˆ™-â‰£ yâ‰£z

  âŸ¨âŸ©-â‰£-syntax : (x : A) {y z : A} â†’ x â‰£ y â†’ y â‰£ z â†’ x â‰£ z
  âŸ¨âŸ©-â‰£-syntax = _âŸ¨_âŸ©-â‰£_
  infixr 2 âŸ¨âŸ©-â‰£-syntax
  infixr 2 _âŸ¨_âŸ©-â‰£_

  infix  3 _âˆ-â‰£

  _âˆ-â‰£ : (x : A) â†’ x â‰£ x
  _ âˆ-â‰£ = refl-â‰£
