
{-# OPTIONS --allow-unsolved-metas #-}

--
-- NOTE: This file is originally from the cubical std library.
--       (https://github.com/agda/cubical)
--       It was copied here to replace references to cubical paths,
--       since cubical agda files cannot currently be compiled to binaries.
--       All copyright belongs to the original authors.
--
-- See:
-- module Cubical.Data.Int.Properties where
--

module Verification.Conventions.Prelude.Data.Int.Properties where

open import Verification.Conventions.Proprelude.CubicalConventions
open import Verification.Conventions.Prelude.Data.Nat.Base hiding (_+_)
open import Verification.Conventions.Prelude.Data.Nat.Properties hiding (+-assoc ; +-comm)
open import Verification.Conventions.Prelude.Data.Int.Base
open import Verification.Conventions.Prelude.Data.Bool.Base
open import Verification.Conventions.Proprelude
open import Verification.Conventions.Prelude.Data.StrictId
open import Verification.Conventions.Prelude.Classes.EquivalenceRelation
open import Verification.Conventions.Prelude.Classes.Setoid
open import Verification.Conventions.Prelude.Classes.Discrete

private
  âŠ¥ = ğŸ˜-ğ’°

{-

This file defines

sucPred : âˆ€ (i : Int) â†’ sucInt (predInt i) â‰£ i
predSuc : âˆ€ (i : Int) â†’ predInt (sucInt i) â‰£ i

discreteInt : discrete Int
isSetInt : isSet Int

addition of Int is defined _+_ : Int â†’ Int â†’ Int

as well as its commutativity and associativity
+-comm : âˆ€ (m n : Int) â†’ m + n â‰£ n + m
+-assoc : âˆ€ (m n o : Int) â†’ m + (n + o) â‰£ (m + n) + o

An alternate definition of _+_ is defined via ua,
namely _+'_, which helps us to easily prove

isEquivAddInt : (m : Int) â†’ isEquiv (Î» n â†’ n + m)

-}


-- open import Cubical.Core.Everything

-- open import Cubical.Foundations.Prelude
-- open import Cubical.Foundations.Equiv
-- open import Cubical.Foundations.Transport
-- open import Cubical.Foundations.HLevels
-- open import Cubical.Foundations.Isomorphism
-- open import Cubical.Foundations.Univalence

-- open import Cubical.Data.Empty
-- open import Cubical.Data.Nat hiding (_+_ ; +-assoc ; +-comm)
-- open import Cubical.Data.Bool
-- open import Cubical.Data.Sum
-- open import Cubical.Data.Int.Base

-- open import Cubical.Relation.Nullary
-- open import Cubical.Relation.Nullary.DecidableEq

abs : Int â†’ â„•
abs (pos n) = n
abs (negsuc n) = suc n

sgn : Int â†’ Bool
sgn (pos n) = true
sgn (negsuc n) = false

sucPred : âˆ€ i â†’ sucInt (predInt i) â‰£ i
sucPred (pos zero)    = refl
sucPred (pos (suc n)) = refl
sucPred (negsuc n)    = refl

predSuc : âˆ€ i â†’ predInt (sucInt i) â‰£ i
predSuc (pos n)          = refl
predSuc (negsuc zero)    = refl
predSuc (negsuc (suc n)) = refl

-- TODO: define multiplication

injPos : âˆ€ {a b : â„•} â†’ pos a â‰£ pos b â†’ a â‰£ b
injPos {a} h = subst-Str T h refl
  where
  T : Int â†’ Typeâ‚€
  T (pos x)    = a â‰£ x
  T (negsuc _) = âŠ¥

injNegsuc : âˆ€ {a b : â„•} â†’ negsuc a â‰£ negsuc b â†’ a â‰£ b
injNegsuc {a} h = subst-Str T h refl
  where
  T : Int â†’ Typeâ‚€
  T (pos _) = âŠ¥
  T (negsuc x) = a â‰£ x

posNotnegsuc : âˆ€ (a b : â„•) â†’ Â¬ (pos a â‰£ negsuc b)
posNotnegsuc a b h = subst-Str T h 0
  where
  T : Int â†’ Typeâ‚€
  T (pos _)    = â„•
  T (negsuc _) = âŠ¥

negsucNotpos : âˆ€ (a b : â„•) â†’ Â¬ (negsuc a â‰£ pos b)
negsucNotpos a b h = subst-Str T h 0
  where
  T : Int â†’ Typeâ‚€
  T (pos _)    = âŠ¥
  T (negsuc _) = â„•

discreteInt : Discrete Int
discreteInt (pos n) (pos m) with discreteâ„• n m
... | yes p = yes (cong-Str pos p)
... | no p  = no (Î» x â†’ p (injPos x))
discreteInt (pos n) (negsuc m) = no (posNotnegsuc n m)
discreteInt (negsuc n) (pos m) = no (negsucNotpos n m)
discreteInt (negsuc n) (negsuc m) with discreteâ„• n m
... | yes p = yes (cong-Str negsuc p)
... | no p  = no (Î» x â†’ p (injNegsuc x))

-- isSetInt : isSet Int
-- isSetInt = Discreteâ†’isSet discreteInt

_â„•-_ : â„• â†’ â„• â†’ Int
a â„•- 0 = pos a
0 â„•- suc b = negsuc b
suc a â„•- suc b = a â„•- b

_+pos_ : Int â†’ â„•  â†’ Int
z +pos 0 = z
z +pos (suc n) = sucInt (z +pos n)

_+negsuc_ : Int â†’ â„• â†’ Int
z +negsuc 0 = predInt z
z +negsuc (suc n) = predInt (z +negsuc n)

_+_ : Int â†’ Int â†’ Int
m + pos n = m +pos n
m + negsuc n = m +negsuc n

_-_ : Int â†’ Int â†’ Int
m - pos zero    = m
m - pos (suc n) = m + negsuc n
m - negsuc n    = m + pos (suc n)

sucInt+pos : âˆ€ n m â†’ sucInt (m +pos n) â‰£ (sucInt m) +pos n
sucInt+pos zero m = refl
sucInt+pos (suc n) m = cong-Str sucInt (sucInt+pos n m)

predInt+negsuc : âˆ€ n m â†’ predInt (m +negsuc n) â‰£ (predInt m) +negsuc n
predInt+negsuc zero m = refl
predInt+negsuc (suc n) m = cong-Str predInt (predInt+negsuc n m)

sucInt+negsuc : âˆ€ n m â†’ sucInt (m +negsuc n) â‰£ (sucInt m) +negsuc n
sucInt+negsuc zero m = (sucPred _) âˆ™ (sym (predSuc _))
sucInt+negsuc (suc n) m = {!!}
-- _ â‰£âŸ¨ sucPred _ âŸ©
--   m +negsuc n                    â‰£[ i ]âŸ¨ predSuc m (~ i) +negsuc n âŸ©
--   (predInt (sucInt m)) +negsuc n â‰£âŸ¨ sym (predInt+negsuc n (sucInt m)) âŸ©
--   predInt (sucInt m +negsuc n) âˆ

predInt+pos : âˆ€ n m â†’ predInt (m +pos n) â‰£ (predInt m) +pos n
predInt+pos zero m = refl
predInt+pos (suc n) m =     {!!}
-- _ â‰£âŸ¨ predSuc _ âŸ©
--   m +pos n                    â‰£[ i ]âŸ¨ sucPred m (~ i) + pos n âŸ©
--   (sucInt (predInt m)) +pos n â‰£âŸ¨ sym (sucInt+pos n (predInt m))âŸ©
--   (predInt m) +pos (suc n)    âˆ

predInt+ : âˆ€ m n â†’ predInt (m + n) â‰£ (predInt m) + n
predInt+ m (pos n) = predInt+pos n m
predInt+ m (negsuc n) = predInt+negsuc n m

+predInt : âˆ€ m n â†’ predInt (m + n) â‰£ m + (predInt n)
+predInt m (pos zero) = refl
+predInt m (pos (suc n)) = (predSuc (m + pos n)) âˆ™ (cong-Str (_+_ m) (sym (predSuc (pos n))))
+predInt m (negsuc n) = refl

sucInt+ : âˆ€ m n â†’ sucInt (m + n) â‰£ (sucInt m) + n
sucInt+ m (pos n) = sucInt+pos n m
sucInt+ m (negsuc n) = sucInt+negsuc n m

+sucInt : âˆ€ m n â†’ sucInt (m + n) â‰£  m + (sucInt n)
+sucInt m (pos n) = refl
+sucInt m (negsuc zero) = sucPred _
+sucInt m (negsuc (suc n)) = (sucPred (m +negsuc n)) âˆ™ (cong-Str (_+_ m) (sym (sucPred (negsuc n))))

pos0+ : âˆ€ z â†’ z â‰£ pos 0 + z
pos0+ (pos zero) = refl
pos0+ (pos (suc n)) = cong-Str sucInt (pos0+ (pos n))
pos0+ (negsuc zero) = refl
pos0+ (negsuc (suc n)) = cong-Str predInt (pos0+ (negsuc n))

negsuc0+ : âˆ€ z â†’ predInt z â‰£ negsuc 0 + z
negsuc0+ (pos zero) = refl
negsuc0+ (pos (suc n)) = (sym (sucPred (pos n))) âˆ™ (cong-Str sucInt (negsuc0+ _))
negsuc0+ (negsuc zero) = refl
negsuc0+ (negsuc (suc n)) = cong-Str predInt (negsuc0+ (negsuc n))

ind-comm : {A : Typeâ‚€} (_âˆ™_ : A â†’ A â†’ A) (f : â„• â†’ A) (g : A â†’ A)
           (p : âˆ€ {n} â†’ f (suc n) â‰£ g (f n))
           (gâˆ™ : âˆ€ a b â†’ g (a âˆ™ b) â‰£ g a âˆ™ b)
           (âˆ™g : âˆ€ a b â†’ g (a âˆ™ b) â‰£ a âˆ™ g b)
           (base : âˆ€ z â†’ z âˆ™ f 0 â‰£ f 0 âˆ™ z)
         â†’ âˆ€ z n â†’ z âˆ™ f n â‰£ f n âˆ™ z
ind-comm _âˆ™_ f g p gâˆ™ âˆ™g base z 0 = base z
ind-comm _âˆ™_ f g p gâˆ™ âˆ™g base z (suc n) = {!!}

  -- z âˆ™ f (suc n) â‰£[ i ]âŸ¨ z âˆ™ p {n} i âŸ©
  -- z âˆ™ g (f n)   â‰£âŸ¨ sym ( âˆ™g z (f n)) âŸ©
  -- g (z âˆ™ f n)   â‰£âŸ¨ cong-Str g IH âŸ©
  -- g (f n âˆ™ z)   â‰£âŸ¨ gâˆ™ (f n) z âŸ©
  -- g (f n) âˆ™ z   â‰£[ i ]âŸ¨ p {n} (~ i) âˆ™ z âŸ©
  -- f (suc n) âˆ™ z âˆ
  -- where
  -- IH = ind-comm _âˆ™_ f g p gâˆ™ âˆ™g base z n

private instance _ = isSetoid:byId

ind-assoc : {A : Typeâ‚€} (_Â·_ : A â†’ A â†’ A) (f : â„• â†’ A)
        (g : A â†’ A) (p : âˆ€ a b â†’ g (a Â· b) â‰£ a Â· (g b))
        (q : âˆ€ {c} â†’ f (suc c) â‰£ g (f c))
        (base : âˆ€ m n â†’ (m Â· n) Â· (f 0) â‰£ m Â· (n Â· (f 0)))
        (m n : A) (o : â„•)
      â†’ m Â· (n Â· (f o)) â‰£ (m Â· n) Â· (f o)
ind-assoc _Â·_ f g p q base m n 0 = sym (base m n)
ind-assoc _Â·_ f g p q base m n (suc o) = {!!}
    -- m Â· (n Â· (f (suc o))) â‰£[ i ]âŸ¨ m Â· (n Â· q {o} i) âŸ©
    -- m Â· (n Â· (g (f o)))   â‰£[ i ]âŸ¨ m Â· (p n (f o) (~ i)) âŸ©
    -- m Â· (g (n Â· (f o)))   â‰£âŸ¨ sym (p m (n Â· (f o)))âŸ©
    -- g (m Â· (n Â· (f o)))   â‰£âŸ¨ cong-Str g IH âŸ©
    -- g ((m Â· n) Â· (f o))   â‰£âŸ¨ p (m Â· n) (f o) âŸ©
    -- (m Â· n) Â· (g (f o))   â‰£[ i ]âŸ¨ (m Â· n) Â· q {o} (~ i) âŸ©
    -- (m Â· n) Â· (f (suc o)) âˆ
    -- where
    -- IH = ind-assoc _Â·_ f g p q base m n o

+-comm : âˆ€ m n â†’ m + n â‰£ n + m
+-comm m (pos n) = ind-comm _+_ pos sucInt refl sucInt+ +sucInt pos0+ m n
+-comm m (negsuc n) = ind-comm _+_ negsuc predInt refl predInt+ +predInt negsuc0+ m n

+-assoc : âˆ€ m n o â†’ m + (n + o) â‰£ (m + n) + o
+-assoc m n (pos o) = ind-assoc _+_ pos sucInt +sucInt refl (Î» _ _ â†’ refl) m n o
+-assoc m n (negsuc o) = ind-assoc _+_ negsuc predInt +predInt refl +predInt m n o

{-
-- Compose sucPathInt with itself n times. Transporting along this
-- will be addition, transporting with it backwards will be subtraction.
-- Use this to define _+'_ for which is easier to prove
-- isEquiv (Î» n â†’ n +' m) since _+'_ is defined by transport

sucPathInt : Int â‰£ Int
sucPathInt = ua (sucInt , isoToIsEquiv (iso sucInt predInt sucPred predSuc))

addEq : â„• â†’ Int â‰£ Int
addEq zero = refl
addEq (suc n) = (addEq n) âˆ™ sucPathInt

predPathInt : Int â‰£ Int
predPathInt = ua (predInt , isoToIsEquiv (iso predInt sucInt predSuc sucPred))

subEq : â„• â†’ Int â‰£ Int
subEq zero = refl
subEq (suc n) = (subEq n) âˆ™ predPathInt

_+'_ : Int â†’ Int â†’ Int
m +' pos n    = transport (addEq n) m
m +' negsuc n = transport (subEq (suc n)) m

+'â‰£+ : _+'_ â‰£ _+_
+'â‰£+ i m (pos zero) = m
+'â‰£+ i m (pos (suc n)) = sucInt (+'â‰£+ i m (pos n))
+'â‰£+ i m (negsuc zero) = predInt m
+'â‰£+ i m (negsuc (suc n)) = predInt (+'â‰£+ i m (negsuc n)) --
  -- compPath (Î» i â†’ (+'â‰£+ i (predInt m) (negsuc n))) (sym (predInt+negsuc n m)) i

isEquivAddInt' : (m : Int) â†’ isEquiv (Î» n â†’ n +' m)
isEquivAddInt' (pos n)    = isEquivTransport (addEq n)
isEquivAddInt' (negsuc n) = isEquivTransport (subEq (suc n))

isEquivAddInt : (m : Int) â†’ isEquiv (Î» n â†’ n + m)
isEquivAddInt = subst-Str (Î» add â†’ (m : Int) â†’ isEquiv (Î» n â†’ add n m)) +'â‰£+ isEquivAddInt'
-}

-- below is an alternate proof of isEquivAddInt for comparison
-- We also have two useful lemma here.

minusPlus : âˆ€ m n â†’ (n - m) + m â‰£ n
minusPlus (pos zero) n = refl
minusPlus (pos 1) = sucPred
minusPlus (pos (suc (suc m))) n = {!!}
  -- sucInt ((n +negsuc (suc m)) +pos (suc m)) â‰£âŸ¨ sucInt+pos (suc m) _ âŸ©
  -- sucInt (n +negsuc (suc m)) +pos (suc m)   â‰£[ i ]âŸ¨ sucPred (n +negsuc m) i +pos (suc m) âŸ©
  -- (n - pos (suc m)) +pos (suc m)            â‰£âŸ¨ minusPlus (pos (suc m)) n âŸ©
  -- n âˆ
minusPlus (negsuc zero) = predSuc
minusPlus (negsuc (suc m)) n = {!!}
  -- predInt (sucInt (sucInt (n +pos m)) +negsuc m) â‰£âŸ¨ predInt+negsuc m _ âŸ©
  -- predInt (sucInt (sucInt (n +pos m))) +negsuc m â‰£[ i ]âŸ¨ predSuc (sucInt (n +pos m)) i +negsuc m âŸ©
  -- sucInt (n +pos m) +negsuc m                    â‰£âŸ¨ minusPlus (negsuc m) n âŸ©
  -- n âˆ

plusMinus : âˆ€ m n â†’ (n + m) - m â‰£ n
plusMinus (pos zero) n = refl
plusMinus (pos (suc m)) = minusPlus (negsuc m)
plusMinus (negsuc m) = minusPlus (pos (suc m))

-- private
--   alternateProof : (m : Int) â†’ isEquiv (Î» n â†’ n + m)
--   alternateProof m = isoToIsEquiv (iso (Î» n â†’ n + m)
--                                        (Î» n â†’ n - m)
--                                        (minusPlus m)
--                                        (plusMinus m))

{-
-}
