
module Verification.Experimental.Algebra.Monoid.Free.Element where

open import Verification.Experimental.Conventions
open import Verification.Experimental.Set.Setoid.Definition
open import Verification.Experimental.Set.Setoid.Free
-- open import Verification.Experimental.Data.Prop.Definition
open import Verification.Experimental.Data.Sum.Definition
open import Verification.Experimental.Algebra.Monoid.Definition
open import Verification.Experimental.Algebra.Monoid.Free.Definition
open import Verification.Experimental.Category.Std.Category.Definition
open import Verification.Experimental.Category.Std.Morphism.Iso

open import Verification.Experimental.Data.Indexed.Definition
open import Verification.Experimental.Data.Indexed.Instance.Monoid
open import Verification.Experimental.Data.Universe.Everything
open import Verification.Experimental.Data.Universe.Instance.Semiring


module _ {A : ğ’° ğ‘–} where

  el : ğ–¥ğ—‹ğ–¾ğ–¾-ğŒğ¨ğ§ A -> ğˆğ± A (ğ”ğ§ğ¢ğ¯ ğ‘–)
  el a = indexed (Î» i â†’ a âˆ i)

  macro
    ğ‘’ğ‘™ = #structureOn el

  private
    lem-1 : âˆ€{a : ğ–¥ğ—‹ğ–¾ğ–¾-ğŒğ¨ğ§ A} -> el (â—Œ â‹† a) â‰… el a
    lem-1 {a} = f since P
      where
        f : el (â—Œ â‹† a) âŸ¶ el a
        f (right-âˆ x) = x

        P = record
            { inverse-â—† = Î» x -> right-âˆ x
            ; inv-r-â—†   = Î» {i (right-âˆ x) â†’ right-âˆ x}
            ; inv-l-â—†   = Î» {_} -> refl
            }

    lem-2 : âˆ€{a : ğ–¥ğ—‹ğ–¾ğ–¾-ğŒğ¨ğ§ A} -> el (a â‹† â—Œ) â‰… el a
    lem-2 {a} = f since P
      where
        f : el (a â‹† â—Œ) âŸ¶ el a
        f (left-âˆ x) = x

        P = record
            { inverse-â—† = Î» x -> left-âˆ x
            ; inv-r-â—†   = Î» {i (left-âˆ x) â†’ left-âˆ x}
            ; inv-l-â—†   = Î» {_} -> refl
            }

    lem-3 : âˆ€{a b c : ğ–¥ğ—‹ğ–¾ğ–¾-ğŒğ¨ğ§ A} -> el (a â‹† b â‹† c) â‰… el (a â‹† (b â‹† c))
    lem-3 {a} {b} {c} = f since P
      where
        f : el (a â‹† b â‹† c) âŸ¶ el (a â‹† (b â‹† c))
        f (left-âˆ (left-âˆ x)) = left-âˆ x
        f (left-âˆ (right-âˆ x)) = right-âˆ (left-âˆ x)
        f (right-âˆ x) = right-âˆ (right-âˆ x)

        g : el (a â‹† (b â‹† c)) âŸ¶ el (a â‹† b â‹† c)
        g (left-âˆ x) = left-âˆ (left-âˆ x)
        g (right-âˆ (left-âˆ x)) = left-âˆ (right-âˆ x)
        g (right-âˆ (right-âˆ x)) = right-âˆ x

        Pâ‚€ : âˆ€{a : A} -> (x : (_ âˆ a)) -> g (f x) â‰¡ x
        Pâ‚€ {a} (left-âˆ (left-âˆ x)) = refl-â‰¡
        Pâ‚€ {a} (left-âˆ (right-âˆ x)) = refl-â‰¡
        Pâ‚€ {a} (right-âˆ x) = refl-â‰¡

        Pâ‚ : âˆ€{a : A} -> (x : (_ âˆ a)) -> f (g x) â‰¡ x
        Pâ‚ {a} (left-âˆ x) = refl-â‰¡
        Pâ‚ {a} (right-âˆ (left-âˆ x)) = refl-â‰¡
        Pâ‚ {a} (right-âˆ (right-âˆ x)) = refl-â‰¡

        P = record
            { inverse-â—† = Î» {_} -> g
            ; inv-r-â—† = Î» {_} -> funExt Pâ‚€
            ; inv-l-â—† = Î» {_} -> funExt Pâ‚
            }

    lem-4 : âˆ€{a b c : ğ–¥ğ—‹ğ–¾ğ–¾-ğŒğ¨ğ§ A} -> (el a â‰… el b) -> el (a â‹† c) â‰… el (b â‹† c)
    lem-4 {a} {b} {c} f = g since P
      where
        g : el (a â‹† c) âŸ¶ el (b â‹† c)
        g (left-âˆ x) = left-âˆ (âŸ¨ f âŸ© x)
        g (right-âˆ x) = right-âˆ x

        h : el (b â‹† c) âŸ¶ el (a â‹† c)
        h (left-âˆ x) = left-âˆ (inverse-â—† (of f) x)
        h (right-âˆ x) = right-âˆ x

        Pâ‚€ : âˆ€{a : A} -> (x : (_ âˆ a)) -> h (g x) â‰¡ x
        Pâ‚€ (left-âˆ x) = cong left-âˆ (Î» i -> inv-r-â—† (of f) i x)
        Pâ‚€ (right-âˆ x) = refl-â‰¡

        Pâ‚ : âˆ€{a : A} -> (x : (_ âˆ a)) -> g (h x) â‰¡ x
        Pâ‚ (left-âˆ x) = cong left-âˆ (Î» i -> inv-l-â—† (of f) i x)
        Pâ‚ (right-âˆ x) = refl-â‰¡

        P = record
            { inverse-â—† = Î» {_} -> h
            ; inv-r-â—†   = Î» {_} -> funExt Pâ‚€
            ; inv-l-â—†   = Î» {_} -> funExt Pâ‚
            }

    lem-5 : âˆ€{a b c : ğ–¥ğ—‹ğ–¾ğ–¾-ğŒğ¨ğ§ A} -> (el a â‰… el b) -> el (c â‹† a) â‰… el (c â‹† b)
    lem-5 {a}{b}{c} f = g since P
      where
        g : el (c â‹† a) âŸ¶ el (c â‹† b)
        g (right-âˆ x) = right-âˆ (âŸ¨ f âŸ© x)
        g (left-âˆ x) = left-âˆ x

        h : el (c â‹† b) âŸ¶ el (c â‹† a)
        h (right-âˆ x) = right-âˆ (inverse-â—† (of f) x)
        h (left-âˆ x) = left-âˆ x

        Pâ‚€ : âˆ€{a : A} -> (x : (_ âˆ a)) -> h (g x) â‰¡ x
        Pâ‚€ (left-âˆ x) = refl-â‰¡
        Pâ‚€ (right-âˆ x) = cong right-âˆ (Î» i -> inv-r-â—† (of f) i x)

        Pâ‚ : âˆ€{a : A} -> (x : (_ âˆ a)) -> g (h x) â‰¡ x
        Pâ‚ (left-âˆ x) = refl-â‰¡
        Pâ‚ (right-âˆ x) = cong right-âˆ (Î» i -> inv-l-â—† (of f) i x)

        P = record
            { inverse-â—† = Î» {_} -> h
            ; inv-r-â—†   = Î» {_} -> funExt Pâ‚€
            ; inv-l-â—†   = Î» {_} -> funExt Pâ‚
            }

    lem-6 : el â—Œ â‰… â—Œ
    lem-6 = f since P
      where
        f : el â—Œ âŸ¶ â—Œ
        f ()

        g : â—Œ âŸ¶ el â—Œ
        g ()

        P = record
            { inverse-â—† = Î» {_} -> g
            ; inv-r-â—†   = Î» {i ()}
            ; inv-l-â—†   = Î» {i ()}
            }

    lem-7 : âˆ€{a b : ğ–¥ğ—‹ğ–¾ğ–¾-ğŒğ¨ğ§ A} -> el (a â‹† b) â‰… el a â‹† el b
    lem-7 {a} {b} = f since P
      where
        f : el (a â‹† b) âŸ¶ el a â‹† el b
        f (left-âˆ x) = left x
        f (right-âˆ x) = right x

        g : el a â‹† el b âŸ¶ el (a â‹† b)
        g (left x) = left-âˆ x
        g (just x) = right-âˆ x

        Pâ‚€ : âˆ€{a : A} -> (x : (_ âˆ a)) -> g (f x) â‰¡ x
        Pâ‚€ (left-âˆ x)  = refl-â‰¡
        Pâ‚€ (right-âˆ x) = refl-â‰¡

        Pâ‚ : âˆ€{a : A} -> (x : (_ âˆ a) + (_ âˆ a)) -> f (g x) â‰¡ x
        Pâ‚ (left x)  = refl-â‰¡
        Pâ‚ (right x) = refl-â‰¡

        P = record
            { inverse-â—† = Î» {_} -> g
            ; inv-r-â—†   = Î» {_} -> funExt Pâ‚€
            ; inv-l-â—†   = Î» {_} -> funExt Pâ‚
            }


  instance
    isSetoidHom:el : isSetoidHom (ğ–¥ğ—‹ğ–¾ğ–¾-ğŒğ¨ğ§ A) (ğˆğ± A (ğ”ğ§ğ¢ğ¯ ğ‘–)) el
    isSetoidHom:el = record { cong-âˆ¼ = rec-RST f}
      where
        f : âˆ€{a b : ğ–¥ğ—‹ğ–¾ğ–¾-ğŒğ¨ğ§ A} -> (a âˆ¼-Free-ğŒğ¨ğ§ b) -> _
        f unit-l-â‹†-Free-ğŒğ¨ğ§ = lem-1
        f unit-r-â‹†-Free-ğŒğ¨ğ§ = lem-2
        f assoc-l-â‹†-Free-ğŒğ¨ğ§ = lem-3
        f (cong-l-â‹†-Free-ğŒğ¨ğ§ p) = lem-4 (f p)
        f (cong-r-â‹†-Free-ğŒğ¨ğ§ p) = lem-5 (f p)

  instance
    isMonoidHom:el : isMonoidHom (ğ–¥ğ—‹ğ–¾ğ–¾-ğŒğ¨ğ§ A) (ğˆğ± A (ğ”ğ§ğ¢ğ¯ ğ‘–)) ğ‘’ğ‘™
    isMonoidHom:el = record
                     { pres-â—Œ = lem-6
                     ; pres-â‹† = lem-7
                     }







