
module Verification.Experimental.Category.Std.Category.Construction.Product where

open import Verification.Conventions
open import Verification.Experimental.Set.Setoid
open import Verification.Experimental.Data.Product.Definition
-- open import Verification.Experimental.Data.Fin.Definition
-- open import Verification.Experimental.Algebra.Monoid.Definition
open import Verification.Experimental.Category.Std.Category.Definition
open import Verification.Experimental.Category.Std.Functor.Definition
open import Verification.Experimental.Category.Std.Morphism.Iso

module _ {A : ð’° ð‘–} {B : ð’° ð‘—} {{_ : isSetoid {ð‘–â‚} A}} {{_ : isSetoid {ð‘—â‚} B}} where
  instance
    isSetoid:Ã— : isSetoid (A Ã— B)
    isSetoid:Ã— = setoid (Î» (aâ‚€ , bâ‚€) (aâ‚ , bâ‚) -> (aâ‚€ âˆ¼ aâ‚) Ã— (bâ‚€ âˆ¼ bâ‚))
                 (refl , refl)
                 (Î» (p , q) -> (p â»Â¹ , q â»Â¹))
                 (Î» (pâ‚€ , qâ‚€) (pâ‚ , qâ‚) -> (pâ‚€ âˆ™ pâ‚ , qâ‚€ âˆ™ qâ‚))

module _ {ð’ž : ð’° ð‘–} {ð’Ÿ : ð’° ð‘—} {{_ : isCategory {ð‘–â‚} ð’ž}} {{_ : isCategory {ð‘—â‚} ð’Ÿ}} where

  instance
    isCategory:Ã— : isCategory (ð’ž Ã— ð’Ÿ)
    isCategory.Hom isCategory:Ã— = Î» (a , b) (c , d) -> (a âŸ¶ c) Ã— (b âŸ¶ d)
    isCategory.isSetoid:Hom isCategory:Ã— = isSetoid:Ã—
    isCategory.id isCategory:Ã—         = id , id
    isCategory._â—†_ isCategory:Ã—        = Î» (fâ‚€ , gâ‚€) (fâ‚ , gâ‚) -> (fâ‚€ â—† fâ‚ , gâ‚€ â—† gâ‚)
    isCategory.unit-l-â—† isCategory:Ã—   = unit-l-â—† , unit-l-â—†
    isCategory.unit-r-â—† isCategory:Ã—   = unit-r-â—† , unit-r-â—†
    isCategory.unit-2-â—† isCategory:Ã—   = unit-2-â—† , unit-2-â—†
    isCategory.assoc-l-â—† isCategory:Ã—  = assoc-l-â—† , assoc-l-â—†
    isCategory.assoc-r-â—† isCategory:Ã—  = assoc-r-â—† , assoc-r-â—†
    isCategory._â—ˆ_ isCategory:Ã—        = Î» (pâ‚€ , qâ‚€) (pâ‚ , qâ‚) -> (pâ‚€ â—ˆ pâ‚ , qâ‚€ â—ˆ qâ‚)

  into-Ã—-â‰… : âˆ€{a b : ð’ž} {c d : ð’Ÿ} -> (p : a â‰… b) (q : c â‰… d) -> (a , c) â‰… (b , d)
  into-Ã—-â‰… p q = (âŸ¨ p âŸ© , âŸ¨ q âŸ©) since P
    where
      P = record
          { inverse-â—†  = (inverse-â—† (of p) , inverse-â—† (of q))
          ; inv-r-â—†    = inv-r-â—† (of p) , inv-r-â—† (of q)
          ; inv-l-â—†    = inv-l-â—† (of p) , inv-l-â—† (of q)
          }


