
module Verification.Core.Data.Tree.Variant.Syntax.Instance.Infer where

open import Verification.Conventions hiding (lookup ; â„•)

open import Verification.Core.Set.AllOf.Setoid
open import Verification.Core.Data.AllOf.Collection.Basics
open import Verification.Core.Data.AllOf.Collection.TermTools
open import Verification.Core.Category.Std.AllOf.Collection.Basics
open import Verification.Core.Category.Std.AllOf.Collection.Limits
open import Verification.Core.Category.Std.AllOf.Collection.Monads

open import Verification.Core.Theory.Std.Inference.Definition
open import Verification.Core.Theory.Std.Inference.Task

open import Verification.Core.Data.Tree.Variant.Syntax.Data
open import Verification.Core.Data.Tree.Variant.Syntax.Definition
open import Verification.Core.Data.Tree.Variant.Syntax.Instance.Monad

open import Verification.Core.Data.Tree.Variant.Token.Data
open import Verification.Core.Data.Tree.Variant.Token.Definition
open import Verification.Core.Data.Tree.Variant.Token.Instance.Monad

module _ {A B : ğ’° ğ‘–} {F : ğ’° ğ‘– -> ğ’° ğ‘–} {{_ : isFunctor (ğ”ğ§ğ¢ğ¯ ğ‘–) (ğ”ğ§ğ¢ğ¯ ğ‘–) F}} where
  _<$>_ : (A -> B) -> F A -> F B
  _<$>_ f x = {!!}



data SyntaxTreeToken : ğ’°â‚€ where
  binder : SyntaxTreeToken

tokenSize-SyntaxTreeToken : SyntaxTreeToken -> â™®â„•
tokenSize-SyntaxTreeToken binder = 2

tokenName-SyntaxTreeToken : SyntaxTreeToken -> Text
tokenName-SyntaxTreeToken binder = "â†¦"

toTokenTreeData : SyntaxTreeData -> TokenTreeData
toTokenTreeData ğ’¹ = record
  { TokenType = SyntaxTreeToken + (TokenType ğ’¹)
  ; tokenSize = either tokenSize-SyntaxTreeToken (Î» xs -> map-List (const tt) (tokenSize ğ’¹ xs))
  ; tokenName = either tokenName-SyntaxTreeToken (tokenName ğ’¹)
  ; tokenList = left binder âˆ· map-List right (tokenList ğ’¹)
  }

private Î´ = toTokenTreeData

module _ {ğ’¹ : SyntaxTreeData} where
  -----------------------------------------
  -- printing of the syntax tree
  mutual

    printáµ˜-SyntaxTreeBindingWithHole : âˆ€ {A} {Î“} {n} -> SyntaxTreeBindingWithHole ğ’¹ A Î“ n -> TokenTree (Î´ ğ’¹) (âˆ‘ A)
    printáµ˜-SyntaxTreeBindingWithHole (skipBinding x) = printáµ˜-SyntaxTree' _ _ x -- hole (_ , x)
    printáµ˜-SyntaxTreeBindingWithHole (incl x) = printáµ˜-SyntaxTreeBinding x

    printáµ˜-SyntaxTreeBinding : âˆ€ {A} {Î“} {n} -> SyntaxTreeBinding ğ’¹ A Î“ n -> TokenTree (Î´ ğ’¹) (âˆ‘ A)
    printáµ˜-SyntaxTreeBinding (incl x) = printáµ˜-SyntaxTree' _ _ x
    -- printáµ˜-SyntaxTreeBinding (hole x rest) = {!!} -- hole (_ , x)
    printáµ˜-SyntaxTreeBinding (bind name x) = node (left binder) ((var name) âˆ· (printáµ˜-SyntaxTreeBinding x) âˆ· [])


    printáµ˜-SyntaxTrees : âˆ€ {A} {Î“} {n} -> DList (SyntaxTreeBindingWithHole ğ’¹ (ix A) Î“) (n)
                                          -> ConstDList (TokenTreeáµ˜ (Î´ ğ’¹) (â¨†áµ˜ A)) (map-List (const tt) n)
    printáµ˜-SyntaxTrees [] = []
    printáµ˜-SyntaxTrees (x âˆ· xs) = printáµ˜-SyntaxTreeBindingWithHole x âˆ· (printáµ˜-SyntaxTrees xs)

    -- NOTE: we need to write the induction without the âˆ‘ on SyntaxTree,
    --       because with it, the termination checker does not see that
    --       the recursion terminates. Hence this implementation version with "'"
    printáµ˜-SyntaxTree' : âˆ€ A i -> (SyntaxTreeáµˆ ğ’¹ A) i -> TokenTree (Î´ ğ’¹) (âˆ‘ A)
    printáµ˜-SyntaxTree' A i (hole x) = hole (i , x)
    printáµ˜-SyntaxTree' A i (var name x) = var name
    printáµ˜-SyntaxTree' A i (node t x) = node (right t) (printáµ˜-SyntaxTrees x)
    printáµ˜-SyntaxTree' A i (annotation a x) = annotation a (printáµ˜-SyntaxTree' A i x)

  printáµ˜-SyntaxTree : âˆ€ A -> â¨† (SyntaxTree ğ’¹ A) -> TokenTree (Î´ ğ’¹) (â¨† A)
  printáµ˜-SyntaxTree A (i , x) = printáµ˜-SyntaxTree' (ix A) i x

  print-SyntaxTree : å¤§MonadHom (_ , SyntaxTree ğ’¹) (_ , TokenTree (Î´ ğ’¹))
  print-SyntaxTree = record { fst = â¨† ; snd = printáµ˜-SyntaxTree since {!!} }


  -----------------------------------------
  -- Parsing from a token tree

  mutual
    parseáµ˜-SyntaxTreeBinding : âˆ€ {A} {Î“} {n}
                           -> (TokenTreeáµ˜ (Î´ ğ’¹) (A))
                           -> Maybe (SyntaxTreeBinding ğ’¹ (ix (å†™ (TokenTree (Î´ ğ’¹) A))) Î“ n)
    parseáµ˜-SyntaxTreeBinding {Î“ = Î“} {n = â¦‹â¦Œ} t = just $ incl (parseáµ˜-SyntaxTree' Î“ t)

    parseáµ˜-SyntaxTreeBinding {Î“ = Î“} {n = tt âˆ· n} (node (left binder) (var name âˆ· (t âˆ· []))) = bind name <$> (parseáµ˜-SyntaxTreeBinding t)
    parseáµ˜-SyntaxTreeBinding {Î“ = Î“} {n = tt âˆ· n} other@(t) = {!!} -- hole (annotation "Expected binder here." other)

    parseáµ˜-SyntaxTrees : âˆ€ {A} {Î“} {n}
                           -> ConstDList (TokenTreeáµ˜ (Î´ ğ’¹) (A)) (map-List (const tt) n)
                           -> DList (SyntaxTreeBindingWithHole ğ’¹ (ix (å†™ (TokenTree (Î´ ğ’¹) A))) Î“) (n)
    parseáµ˜-SyntaxTrees {n = â¦‹â¦Œ} [] = []
    parseáµ˜-SyntaxTrees {n = _ âˆ· _} (x âˆ· xs) =
      either (const (skipBinding (hole x))) incl (parseáµ˜-SyntaxTreeBinding x)
      âˆ· parseáµ˜-SyntaxTrees xs


    parseáµ˜-SyntaxTree' : âˆ€ {A} -> (Î“ : äººList Text) -> TokenTree (Î´ ğ’¹) A -> (ix (SyntaxTree ğ’¹ (å†™ (TokenTree (Î´ ğ’¹) A))) Î“)
    parseáµ˜-SyntaxTree' Î“ (hole x) = hole (hole x)
    parseáµ˜-SyntaxTree' Î“ (var x) = case find-first-âˆ Î“ x of
                                           (Î» p -> hole (annotation ("The variable " <> x <> " is not in scope") (var x)))
                                           (Î» Î“âˆx â†’ var x Î“âˆx)
    parseáµ˜-SyntaxTree' Î“ (node (left binder) x) = hole (annotation "No variable binding allowed here." ((node (left binder) x)))
    parseáµ˜-SyntaxTree' Î“ (node (just t) x) = node t (parseáµ˜-SyntaxTrees x)
    parseáµ˜-SyntaxTree' Î“ (annotation a x) = annotation a (parseáµ˜-SyntaxTree' Î“ x)

  parseáµ˜-SyntaxTree : âˆ€ A -> TokenTree (Î´ ğ’¹) A -> (â¨† (SyntaxTree ğ’¹ (å†™ (TokenTree (Î´ ğ’¹) A))))
  parseáµ˜-SyntaxTree A t = _ , parseáµ˜-SyntaxTree' â—Œ t


  -----------------------------------------
  -- This gives us an inference morphism

  isInferHom:print-SyntaxTree : isInferHom print-SyntaxTree
  isInferHom:print-SyntaxTree = record
    { inferF = å†™
    ; infer = parseáµ˜-SyntaxTree since {!!}
    ; eval-infer = {!!}
    }

  infer-SyntaxTree : SyntaxTreeInfer ğ’¹ âŸ¶ TokenTreeInfer (Î´ ğ’¹)
  infer-SyntaxTree = subcathom print-SyntaxTree isInferHom:print-SyntaxTree



